Spacetalk/Step.lean
@@ -38,7 +38,7 @@ inductive Prog : List Ty → Ty → Type
   | const : (α : Ty) → Prog [α] α
   | zip : BinaryOp α β γ → Prog aInp α → Prog bInp β → Prog (aInp ++ bInp) γ
   | map : UnaryOp α β → Prog inp α → Prog inp β
-  | reduce : BinaryOp α β α → (len : Nat) → 0 < len → α.denote → Prog inp β → Prog inp α
+  | reduce : BinaryOp α β α → Nat → α.denote → Prog inp β → Prog inp α
 
 ------------------ Semantics ------------------
 def BinaryOp.denote : BinaryOp α β γ → α.denote → β.denote → γ.denote
@@ -53,6 +53,6 @@ def Prog.denote {inputs : List Ty} {α : Ty} : Prog inputs α → (DenoStreamsLi
   | .const _ => λ ([a]ₕ) ↦ [a]ₕ
   | .zip op as bs => λ inp ↦ let (aInp, bInp) := inp.split; [Stream'.zip op.denote (as.denote aInp).head (bs.denote bInp).head]ₕ
   | .map op as => λ inp ↦ [Stream'.map op.denote (as.denote inp).head]ₕ
-  | .reduce op n _ init bs => λ inp ↦ [Stream'.reduce op.denote n init (bs.denote inp).head]ₕ
+  | .reduce op n init bs => λ inp ↦ [Stream'.reduce op.denote n init (bs.denote inp).head]ₕ
 
 end Step
