lakefile.lean
@@ -4,7 +4,8 @@ open Lake DSL
 package «spacetalk» where
   -- add any package configuration options here
 
-require std from git "https://github.com/leanprover/std4" @ "main"
+require batteries from
+  git "https://github.com/leanprover-community/batteries" @ "main"
 
 require mathlib from git
   "https://github.com/leanprover-community/mathlib4.git"
